compiler/src/compiler/FlatToRiscvSimulation.v
@@ -70,6 +70,7 @@ Section Sim.
       regs_initialized regs1 -> regs_initialized regs2.
 
   Lemma flatToRiscvSim{hyps: @FlatToRiscv.assumptions p}: forall (g: GhostConsts) (pos: Z),
+      NoDup g.(funnames) ->
       simulation FlatImp.SimExec FlatToRiscvCommon.runsTo (related g pos).
   Proof.
     unfold simulation, FlatImp.SimExec, related, FlatImp.SimState.
@@ -95,6 +96,7 @@ Section Sim.
       + assumption.
       + assumption.
       + ring_simplify (pos + 0). reflexivity.
+      + assumption.
       + assumption.
       + assumption.
     - simpl. intros. simp.
