compiler/src/compiler/ProgramSpec.v
@@ -42,6 +42,8 @@ Section Params1.
                 Prop)
          (spec: ProgramSpec): Prop :=
   {
+    funnames_NoDup: NoDup prog.(funnames);
+
     init_code_correct: forall m0 mc0,
       mem_available spec.(datamem_start) spec.(datamem_pastend) m0 ->
       exec prog.(funimpls) prog.(init_code) nil m0 map.empty mc0
